theories/Tests.v
@@ -3,14 +3,41 @@ From Ceres Require Import Ceres.
 From Malfunction Require Import Pipeline Serialize.
 
 From MetaCoq Require Import ETransform Transform bytestring.
-From MetaCoq.Template Require Import All Loader.
+From MetaCoq.Template Require All Loader TemplateMonad.
 
 Import Transform.
+
+Definition eval_malfunction (cf := config.extraction_checker_flags) (p : Ast.Env.program)
+  : String.string :=
+  let p' := run malfunction_pipeline p (MCUtils.todo "wf_env and welltyped term"%bs) in
+  let t := Malfunction.Mlet (MCList.rev_map Malfunction.Named (fst p'), snd p') in
+  time "Pretty printing"%bs (@to_string _ Serialize_t) t.
 
 Definition compile_malfunction {cf : config.checker_flags} (p : Ast.Env.program)
   : String.string :=
   let p' := run malfunction_pipeline p (MCUtils.todo "wf_env and welltyped term"%bs) in
-  time "Pretty printing"%bs to_string  p'.
+  time "Pretty printing"%bs (@to_string _ Serialize_program) p'.
+
+Section something.
+
+Import Loader All.
+Import MCMonadNotation.
+
+Definition extract {A : Type} (a : A) :=
+  t <- tmQuoteRec a ;;
+  s <- tmEval lazy (eval_malfunction t) ;;
+  (* tmMsg "Extraction to Malfunction:"%bs ;; *)
+  tmMsg (String.of_string s) ;; tmReturn tt.
+
+End something.
+
+Notation "'Extraction' a" :=
+  (extract a) (at level 1, a at level 2).
+
+Inductive three := ZERO | ONE | TWO | THREE.
+
+MetaCoq Run Extraction (match cons THREE nil with cons x _ => x | _ => ONE end).
+MetaCoq Run Extraction plus.
 
 Fixpoint ack (n m:nat) {struct n} : nat :=
   match n with
@@ -22,14 +49,43 @@ Fixpoint ack (n m:nat) {struct n} : nat :=
                  end
              in ackn m
   end.
-Definition ack35 := (ack 3 5).
 
-MetaCoq Quote Recursively Definition cbv_ack35 :=
-  ltac:(let t:=(eval cbv delta in (
+MetaCoq Run Extraction (ack 3 5).
 
-                   ack 3 5
+MetaCoq Run Extraction (@exist _ _ 0 (@eq_refl _ 0) : {x : nat | x = 0}).
 
-               ))
-        in exact t).
-Compute (compile_malfunction cbv_ack35).
+Definition vplus {n:nat} :
+  Vector.t nat n -> Vector.t nat n -> Vector.t nat n := (Vector.map2 plus).
+Definition v01 : Vector.t nat 2 :=
+  (Vector.cons nat 0 1 (Vector.cons nat 1 0 (Vector.nil nat))).
+Definition v23 : Vector.t nat 2 :=
+  (Vector.cons nat 2 1 (Vector.cons nat 3 0 (Vector.nil nat))).
+Definition vplus0123 := Vector.hd (vplus v01 v23).
 
+MetaCoq Run Extraction vplus0123.
+
+Inductive tree (A:Set) : Set :=
+  node : A -> forest A -> tree A
+with forest (A:Set) : Set :=
+     | leaf : A -> forest A
+     | fcons : tree A -> forest A -> forest A.
+Arguments leaf {A}.
+Arguments fcons {A}.
+Arguments node {A}.
+
+Fixpoint tree_size (t:tree bool) : nat :=
+  match t with
+    | node a f => S (forest_size f)
+  end
+with forest_size (f:forest bool) : nat :=
+       match f with
+         | leaf b => 1
+         | fcons t f1 => (tree_size t + forest_size f1)
+       end.
+
+Definition arden: forest bool :=
+  fcons (node true (fcons (node true (leaf false)) (leaf true)))
+        (fcons (node true (fcons (node true (leaf false)) (leaf true)))
+               (leaf false)).
+
+MetaCoq Run Extraction (forest_size arden).
